\begin{homeworkProblem}

Let $T: V \mapsto W$ be a linear transformation. Prove the following results:

\begin{enumerate}
  \item $N(T) = N(-T)$.
  \item $N(T^k) = N((-T)^k)$.
  \item If $V = W$ (so that $T$ is a linear operator on $V$) and $\lambda$ is an eigenvalue of $T$, then for any positive integer $k$,
  \[
    N((T - \lambda I_V)^k) = N((-T + \lambda I_V)^k).
  \]
\end{enumerate}

\solution

\begin{enumerate}
  \item $T(x) = 0 \Longleftrightarrow -T(x) = 0 \Longleftrightarrow (-T)(x) = 0$, which means that $N(T) = N(-T)$.
  \item $T^k(x) = 0 \Longleftrightarrow (-1)^k T^k (x) = 0 \Longleftrightarrow (-T)^k (x) = 0$, which means that $N(T^k) = N((-T)^k)$
  \item Since (b) holds, $N((T-\lambda I_V)^k) = N((-(\lambda I_V - T))^k) = N((\lambda I_V - T)^k)$
\end{enumerate}

\end{homeworkProblem}
