\begin{homeworkProblem}
<<<<<<< HEAD

Let $A$ and $B$ be $n \times n$ matrices. Recall that the trace of $A = (a_{ij})$ is defined by $tr(A) = \sum_{i=1}^{n} a_{ii}$. Prove that $tr(AB) = tr(BA)$.
=======
Let $x = (2, 1+i, i)$ and $y = (2-i, 2, 1+2i)$ be vectors in $\mathbb{C}^3$.
Compute $\langle x, y \rangle$, $\norm{x}$, $\norm{y}$, and $\norm{x + y}$.
Then verify both the Cauchy-Schwarz inequality and triangle inequality.
>>>>>>> 3fba870 (Finish all problems)

\solution

<<<<<<< HEAD
\begin{proof}
=======
\part: Compute $\langle x, y \rangle$, $\norm{x}$, $\norm{y}$, and $\norm{x + y}$

\[
\begin{aligned}
\left\langle x, y \right\rangle &=
\sum_{i=1}^{n}x_i \overline{y_i}\\
&= 2 \cdot (2+i) + (1+i) \cdot 2 + i \cdot (1-2i) \\
&= (4 + 2i) + (2 + 2i) + i + 2\\
&= \boxed{8 + 5i}
\end{aligned}
\]

\[
\begin{aligned}
\norm{x} &= \sqrt{\langle x, x\rangle} \\
&= \sqrt{2^2 + (1+i)(1-i) + i\cdot(-i)}\\
&= \boxed{\sqrt{7}}
\end{aligned}
\]

\[
\begin{aligned}
\norm{y} &= \sqrt{\langle y, y \rangle} \\
&= \sqrt{(2-i)(2+i) + 2^2 + (1+2i)(1-2i)} \\
&= \boxed{\sqrt{14}}
\end{aligned}
\]

\[
\begin{aligned}
\norm{x + y} &= \sqrt{\langle x+y, x+y \rangle} \\
&= \sqrt{(4-i)(4+i) + (3+i)(3-i) + (1+3i)(1-3i)} \\
&= \boxed{\sqrt{37}}
\end{aligned}
\]

\part: Verify Cauchy-Schwarz inequality and triangle inequality

By Cauchy-Schwarz inequality, $\langle x, y \rangle \leq \norm{x} \cdot \norm{y}$.
Verify:
\[
|\langle x, y \rangle| = \sqrt{8^2 + 5^2} = \sqrt{89} \leq \norm{x}\cdot\norm{y} = \sqrt{7}\sqrt{14} = \sqrt{98}
\]

By triangle inequality, $\norm{x + y} \leq \norm{x} + \norm{y}$. Verify:
\[
\norm{x + y} = \sqrt{37} \leq \norm{x} + \norm{y} = \sqrt{7} + \sqrt{14}
\]
>>>>>>> 3fba870 (Finish all problems)

Let $A = (a_{ij})$, $B = (b_{ij})$, AB = $(\alpha_{ij})$ and BA = $(\beta_{ij})$.

By the definition of matrix multiplication, we have
\[
    \alpha_{ij} = (\sum_{k=1}^{n} a_{ik} b_{kj}), \text{ and }
    \beta_{ij} = (\sum_{k=1}^{n}b_{ik} a_{kj})
\]

It's trivial to see that
\[
\begin{aligned}
    tr(AB) &= \sum_{i=1}^{n} \alpha_{ii} \\
           &= \sum{i=1}^{n}\left(\sum_{k=1}^{n}a_{ik}b_{kj}\right)
\end{aligned}
\]
\[
\begin{aligned}
    tr(BA) &= \sum_{i=1}^{n} \beta_{ii} \\
           &= \sum_{i=1}^{n}\left(\sum_{k=1}^{n}b_{ik}a_{kj}\right)
\end{aligned}
\]
Thus, $tr(AB) = tr(BA)$.

\end{proof}
\end{homeworkProblem}
