\begin{homeworkProblem}

Let $T$ be a self-adjoint linear operator on a finite-dimensional inner product
space. Prove that $(T + iI)(T - iI)^{-1}$ is unitary using the following conclusion:
$T - iI$ is invertible and $[(T -iI)^{-1}]^* = (T + iI)^{-1}$ if $T$ is self-adjoint.

\solution

\begin{proof}
Linear operator $T$ is unitary if $TT^* = T^*T = I$.

\[
\begin{aligned}
&\phantom{= } [(T + iI)(T - iI)^{-1}]^*[(T + iI)(T - iI)^{-1}]\\
&= [(T-iI)-1]^*(T+iI)^*(T+iI)(T-iI)^{-1}\\
&= (T+iI)^{-1}(T+iI)(T-iI)(T-iI)^{-1}\\
&=I
\end{aligned}
\]
\end{proof}
\end{homeworkProblem}
