\begin{homeworkProblem}
Let $A$ and $B$ be $n \times n$ matrices such that $AB$ is invertible. Prove that $A$ and $B$ are invertible.

\solution

<<<<<<< HEAD
\begin{proof}

Let $C = B(AB)^{-1}$ and $D = (AB)^{-1}A$. Then we have
\[
\begin{aligned}
    AC &= A(B(AB)^{-1}) \\
       &= (AB)(AB)^{-1} \\
       &= I
\end{aligned}
\]

It's trivial to see that $CA = I$ because
\[\begin{aligned}
    I &= CC^{-1} \\
      &= CIC^{-1} \\
      &= C(AC)C^{-1} \\
      &= (CA)(CC^{-1}) \\
      &= CA
\end{aligned}\]

Since $AC = CA = I$, $C = A^{-1}$, which means $A$ is invertible.

Also we have
\[\begin{aligned}
    DB &= ((AB)^{-1}A)B \\
       &= (AB)^{-1}(AB) \\
       &= I
\end{aligned}\]
By the proof elaborated above, we know that $D = B^{-1}$, which means $B$ is invertible.
=======
\part: Compute $\langle x, y \rangle$, $\norm{x}$, $\norm{y}$, and $\norm{x + y}$

\[
\begin{aligned}
\left\langle x, y \right\rangle &=
\int_0^1{f(t)g(t)}\dt \\
&= t e^t \Bigr|_{0}^{1} + \int_0^1{e^t}\dt \\
&= e - e^t \Bigr|_{0}^{1} \\
&= \boxed{1}
\end{aligned}
\quad\ \quad
\begin{aligned}
\norm{f} &= \sqrt{\langle f, f\rangle} \\
&= \sqrt{\int_0^1 t^2 \dt} = \sqrt{\eval{\frac{1}{3}t^3}{0}{1}}\\
&= \boxed{\frac{\sqrt{3}}{3}}
\end{aligned}
\]
\[
\begin{aligned}
\norm{g} &= \innerprod[g]{g} \\
&= \sqrt{\int_0^1 e^{2t} \dt} = \sqrt{\eval{\frac{1}{2}te^{2t}}{0}{1}} \\
&= \boxed{\sqrt{\frac{1}{2}e^2 - \frac{1}{2}}}
\end{aligned}
\quad\ \quad
\begin{aligned}
\norm{f + g} &= \innerprod[t + e^t]{t + e^t} \\
&= \sqrt{\int_0^1 e^{2t} + t^2 + 2te^t \dt}\\
&= \sqrt{\int_0^1 e^{2t} \dt + \int_0^1 t^2 \dt + 2 \int_0^1 t e^t \dt} \\
&= \boxed{\sqrt{\frac{1}{2}e^2 + \frac{11}{6}}}
\end{aligned}
\]

\part: Verify Cauchy-Schwarz inequality and triangle inequality

By Cauchy-Schwarz inequality, $\langle f, g \rangle \leq \norm{f} \cdot \norm{g}$.
Verify:
\[
|\innerprod[f]{g}| = 1 \leq \norm{f}\cdot\norm{g} = \frac{\sqrt{3}}{3} \cdot \sqrt{\frac{1}{2}e^2 - \frac{1}{2}} = \sqrt{\frac{1}{6} e^2 - \frac{1}{6}} \approx 1.065
\]

By triangle inequality, $\norm{f + g} \leq \norm{f} + \norm{g}$. Verify:
\[
\norm{f + g} = \sqrt{\frac{1}{2}e^2 + \frac{11}{6}} \approx 2.35 \leq \norm{f} + \norm{g} = \sqrt{\frac{1}{2}e^2 - \frac{1}{6}} \approx 2.63
\]

>>>>>>> 3fba870 (Finish all problems)

So, we have proven when $AB$ is invertible, $A$ and $B$ are both invertible.
\end{proof}
\end{homeworkProblem}
