\begin{homeworkProblem}
\solution
\[
A e_1' = \begin{pmatrix}
    1 & 1 & -1 \\
    2 & 0 & 1 \\
    1 & 1 & 0
\end{pmatrix}
\begin{pmatrix}
    1 \\
    1 \\
    1
\end{pmatrix} = \begin{pmatrix}
    1 \\
    3 \\
    2
\end{pmatrix}\\
A e_2' = \begin{pmatrix}
    1 & 1 & -1 \\
    2 & 0 & 1 \\
    1 & 1 & 0
\end{pmatrix}
\begin{pmatrix}
    1 \\
    0 \\
    1
\end{pmatrix} = \begin{pmatrix}
    0 \\
    3 \\
    1
\end{pmatrix}\\
A e_3' = \begin{pmatrix}
    1 & 1 & -1 \\
    2 & 0 & 1 \\
    1 & 1 & 0
\end{pmatrix}
\begin{pmatrix}
    1 \\
    1 \\
    2
\end{pmatrix} = \begin{pmatrix}
    0 \\
    4 \\
    2
\end{pmatrix}
\]
Suppose $A' = \left( \begin{smallmatrix}a_1 & a_2 & a_3 \\ b_1 & b_2 & b_3 \\ c_1 & c_2 & c_3 \end{smallmatrix} \right)$, then we know that
\[
\begin{pmatrix}
    1 \\
    3 \\
    2
\end{pmatrix}
= a_1\vec{\boldmath{e_1}}' + b_1\vec{\boldmath{e_2}}' + c_1 \vec{\boldmath{e_3}}'
= \begin{pmatrix}
    a_1 + b_1 + c_1 \\
    a_1 + c_1 \\
    a_1 + b_1 + 2c_1
\end{pmatrix}
\]\[
\begin{pmatrix}
    0 \\
    3 \\
    1
\end{pmatrix}
= a_2\vec{\boldmath{e_1}}' + b_2\vec{\boldmath{e_2}}' + c_2 \vec{\boldmath{e_3}}'
= \begin{pmatrix}
    a_2 + b_2 + c_2 \\
    a_2 + c_2 \\
    a_2 + b_2 + 2c_2
\end{pmatrix}
 \]

 \[
\begin{pmatrix}
    0 \\
    4 \\
    2
\end{pmatrix}  a_3\vec{\boldmath{e_1}}' + b_3\vec{\boldmath{e_2}}' + c_3\vec{\boldmath{e_3}}'
= \begin{pmatrix}
    a_3 + b_3 + c_3 \\
    a_3 + c_3 \\
    a_3 + b_3 + 2c_3
\end{pmatrix}
\]

We solve that \[
A' = \begin{pmatrix}
     4 &  2 &  2 \\
    -2 & -3 & -4 \\
    -1 &  1 &  2
\end{pmatrix}\]
\end{homeworkProblem}
