\begin{homeworkProblem}

\solution
<<<<<<< HEAD

\begin{proof}
Proving $\det(A) = 0$ is equivalent to proving $A$ is not invertible. Suppose that $A$ is invertible, then we have \[
    AA^{-1} = I
\]
It's trivial to see that when $A$ is nilpotent, we have \[
\begin{aligned}
    (AA^{-1})^{k} &= I \\
    (A^{k})(A^{-k}) &= I \\
    O A^{-k} &= I \\
    O &= I
\end{aligned}
\]
This can never happen. By contradiction we have proven that $A$ is not invertible, thus $\det(A) = 0$ when $A$ is nilpotent.
\end{proof}
=======
\begin{enumerate}
    \item \begin{proof}
\[
\begin{aligned}
T_1^* &= \left(\frac{1}{2}(T + T^*)\right)^* \\
&= \frac{1}{2}(T^* + (T^*)^*)\\
&= \frac{1}{2}(T^* + T) \\
&= T_1
\end{aligned}
\quad \, \quad
\begin{aligned}
T_2^* &= \left(\frac{1}{2i}(T - T^*)\right)^* \\
&= \frac{1}{2i}(T^* - (T^*)^*) \\
&= \frac{1}{2i}(-T^* + T) \\
&= T_2
\end{aligned}
\]
\[T_1 + iT_2 = \frac{1}{2} (T + T^*) + \frac{1}{2}(T - T^*) = T \]
\end{proof}
\item \begin{proof}
    If $T = U_1 + i U_2$ and $U_1$, $U_2$ are self-adjoint, then
    \[
        T^* = (U_1 + iU_2)^* = U_1^* - iU_2^* = U_1 - iU_2
    \]
    \[
        T_1^* = \left(\frac{1}{2}(T + T^*)\right)= \frac{1}{2}((U_1 + iU_2) + (U_1 - iU_2)) = U_1
    \]
    \[
        T_1^* = \left(\frac{1}{2i}(T - T^*)\right)= \frac{1}{2i}((U_1 + iU_2) - (U_1 - iU_2)) = U_2
    \]
\end{proof}
\item \begin{proof}
\[
T_1T_2 = \frac{1}{2}(T + T^*)\frac{1}{2i}(T - T^*) = \frac{1}{4i}(T^2 - TT^* + T^*T - (T^*)^2)
\]
\[
T_2T_1 = \frac{1}{2i}(T - T^*)\frac{1}{2}(T + T^*) = \frac{1}{4i}(T^2 + TT^* - T^*T - (T^*)^2)
\]
If $T_1T_2 = T_2 T_1$, then \[
    \frac{1}{4i}(T^2 - TT^* + T^*T - (T^*)^2) = \frac{1}{4i}(T^2 + TT^* - T^*T - (T^*)^2)
\] which is equivalent to \[
2T^*T = TT^* \Longrightarrow T \text{ is normal}
\]
If $T$ is normal, then $T_1T_2 = T_2T_1$
\end{proof}
\end{enumerate}

>>>>>>> 3fba870 (Finish all problems)
\end{homeworkProblem}
